Redefined all operators to bigi definition, and added corresponding lemmas.

Security/SaberRqPreliminaries.ec
@@ -3,7 +3,7 @@
 (* ------------------------------------------------------------------------------------- *)
 
 (* --- Built-in --- *)
-require import AllCore List Distr Ring ZModP IntDiv Bigalg StdOrder.
+require import AllCore List Distr DInterval DList Ring ZModP IntDiv Bigalg StdOrder.
 require (*--*) Matrix PKE.
 (*---*) import IntOrder.
 
@@ -113,6 +113,7 @@ proof.
   rewrite -exprD_nneg; first 2 by rewrite (lez_trans 2 0 ep); [| apply ge2_ep || apply ge2_ep ].
    by congr; rewrite -addzA /= mulzC -mul1r2z /ofint_id intmulz.
 qed.
+
 
 (* --- Types, Operators and Distributions --- *)
 abstract theory PolyZ.
@@ -320,16 +321,259 @@ import Z2t R2t R2t.ComRing R2t.BasePoly.
 import Z2 R2 R2.ComRing R2.BasePoly.
 import Rp.BasePoly.BigCf.
 
-(* - From Rq to Rp - *)
-op Zq2Zp (z : Zq) : Zp =
-  Zp.inzmod (asint z).
+(* - Constants - *)
+const h1 : Rq = pi (to_polyd (fun _ => Zq.inzmod (2 ^ (eq - ep - 1)))).
+const h2 : Rq = pi (to_polyd (fun _ => Zq.inzmod (2 ^ (ep - 2) - 2 ^ (ep - et - 2)))).
+const h : Rq_vec = vectc h1.
 
+(* -- Cryptographic Types and Distributions  -- *)
+type seed.
+type pkey.
+type skey.
+type plaintext.
+type ciphertext.
+
+op [lossless full uniform] dseed : seed distr.
+
+(* -- Operations -- *)
+op gen : seed -> Rq_mat.
+
+(* - Modular Reduction/Modulus Conversion - *)
+op Zq2Zp (z : Zq) : Zp = Zp.inzmod (asint z).
+op Zp2Zq (z : Zp) : Zq = Zq.inzmod (Zp.asint z).
+op Zp2Zppq (z : Zp) : Zppq = Zppq.inzmod (Zp.asint z).
+
+(* Lift Modular Reduction/Modulus Conversion to Polynomials *)
+op Rq2Rp (p : Rq) : Rp =
+  BigRp.XnD1CA.bigi predT (fun (i : int) => Zq2Zp p.[i] ** exp Rp.iX i) 0 n.
+op Rp2Rq (p : Rp) : Rq =
+  BigRq.XnD1CA.bigi predT (fun (i : int) => Zp2Zq p.[i] ** exp Rq.iX i) 0 n.
+op Rp2Rppq (p : Rp) : Rppq =
+  BigRppq.XnD1CA.bigi predT (fun (i : int) => Zp2Zppq p.[i] ** exp Rppq.iX i) 0 n.
+
+(* Lift Modular Reduction/Modulus Conversion to Polynomial Vectors *)
+op Rqv2Rpv (p : Rq_vec) : Rp_vec = offunv (fun (i : int) => Rq2Rp p.[i]).
+op Rpv2Rqv (pv : Rp_vec) : Rq_vec = offunv (fun (i : int) => Rp2Rq pv.[i]).
+
+(* - Scaling (Bit-shift + Modulus Conversion) - *)
+op shl (x : int, ex : int) : int = x * 2 ^ ex.
+op shr (x : int, ex : int) : int = x %/ 2 ^ ex.
+op shl_enc (x : R2, ex : int) : Rp =  
+  BigRp.XnD1CA.bigi predT (fun (i : int) => 
+  Zp.inzmod (shl (Z2.asint x.[i]) ex) ** exp Rp.iX i) 0 n.   
+op shl_dec (x : R2t) : Rp =
+  BigRp.XnD1CA.bigi predT (fun (i : int) => 
+  Zp.inzmod (shl (Z2t.asint x.[i]) (ep - et - 1)) ** exp Rp.iX i) 0 n.
+
+op scale (x : int, ea : int, eb : int) : int = shr x (ea - eb).
+
+op scaleZq2Zp (z : Zq) : Zp = Zp.inzmod (scale (Zq.asint z) eq ep).
+op scaleZp2Zp (z : Zp) : Zp = Zp.inzmod (scale (Zp.asint z) ep ep).
+op scaleZp2Zppq (z : Zp) : Zppq = Zppq.inzmod (scale (Zp.asint z) ep (2 * ep - eq)).
+op scaleZp2Z2t (z : Zp) : Z2t = Z2t.inzmod (scale (Zp.asint z) ep (et + 1)).
+op scaleZp2Z2 (z : Zp) : Z2 = Z2.inzmod (scale (Zp.asint z) ep 1).
+op scaleZppq2Z2t (z : Zppq) : Z2t = Z2t.inzmod (scale (Zppq.asint z) (2 * ep - eq) (et + 1)).
+
+(* Lift Scaling to Polynomials *)
+op scaleRq2Rp (p : Rq) : Rp = 
+  BigRp.XnD1CA.bigi predT (fun (i : int) => scaleZq2Zp p.[i] ** exp Rp.iX i) 0 n.
+op scaleRp2Rp (p : Rp) : Rp = 
+  BigRp.XnD1CA.bigi predT (fun (i : int) => scaleZp2Zp p.[i] ** exp Rp.iX i) 0 n.
+op scaleRp2Rppq (p : Rp) : Rppq = 
+  BigRppq.XnD1CA.bigi predT (fun (i : int) => scaleZp2Zppq p.[i] ** exp Rppq.iX i) 0 n.
+op scaleRp2R2t (p : Rp) : R2t = 
+  BigR2t.XnD1CA.bigi predT (fun (i : int) => scaleZp2Z2t p.[i] ** exp R2t.iX i) 0 n.
+op scaleRp2R2 (p : Rp) : R2 = 
+  BigR2.XnD1CA.bigi predT (fun (i : int) => scaleZp2Z2 p.[i] ** exp R2.iX i) 0 n.
+op scaleRppq2R2t (p : Rppq) : R2t = 
+  BigR2t.XnD1CA.bigi predT (fun (i : int) => scaleZppq2Z2t p.[i] ** exp R2t.iX i) 0 n.
+
+(* Lift Scaling to Polynomial Vectors *)
+op scaleRqv2Rpv (pv : Rq_vec) : Rp_vec = offunv (fun (i : int) => scaleRq2Rp pv.[i]).
+
+(* - Encoding/Decoding - *)
+op pk_encode ['a] : 'a -> pkey.
+op pk_decode ['a] : pkey -> 'a.
+
+op sk_encode ['a] : 'a -> skey.
+op sk_decode ['a] : skey -> 'a.
+
+op m_encode ['a] : 'a -> plaintext.
+op m_decode ['a] : plaintext -> 'a.
+
+op c_encode ['a] : 'a -> ciphertext.
+op c_decode ['a] : ciphertext -> 'a.
+
+(* - Properties - *)
+(* Encoding and Decoding are Each Other's Inverses *)
+axiom pk_enc_dec_inv ['a] (x : 'a) : pk_decode (pk_encode x) = x. 
+axiom sk_enc_dec_inv ['a] (x : 'a) : sk_decode (sk_encode x) = x. 
+axiom m_enc_dec_inv ['a] (x : 'a) : m_decode (m_encode x) = x. 
+axiom c_enc_dec_inv ['a] (x : 'a) : c_decode (c_encode x) = x. 
+
+(* Modular Reduction/Modulo Conversion *)
 lemma Zq2Zp0 : Zq2Zp Zq.zero = Zp.zero.
-proof. by rewrite -eq_inzmod zeroE mod0z. qed.
+proof. by rewrite -eq_inzmod zeroE. qed.
 
-import DInterval DList.
+lemma Zp2Zq0 : Zp2Zq Zp.zero = Zq.zero.
+proof. by rewrite -eq_inzmod zeroE. qed.
 
-lemma duni_Zp_Zq : dmap DZqP.dunifin Zq2Zp = DZpP.dunifin.
+lemma Zp2Zppq0 : Zp2Zppq Zp.zero = Zppq.zero.
+proof. by rewrite -eq_inzmod zeroE. qed.
+
+lemma Zq2Zp_DM (a b : Zq) : morphism_2 Zq2Zp Zq.( + ) Zp.( + ).
+proof. by move => x y; rewrite /Zq2Zp /( + ) !inzmodK /inzmod modzDm modz_dvd 1:p_div_q. qed.
+
+lemma Zq2Zp_BM (a b : Zq) : morphism_2 Zq2Zp Zq.( - ) Zp.( - ).
+proof. 
+by move => x y; rewrite /Zq2Zp /( + ) !inzmodK modzNm /inzmod modzDm modzDmr modz_dvd 1:p_div_q. 
+qed.
+
+lemma Zq2Zp_MM (a b : Zq) : morphism_2 Zq2Zp Zq.( * ) Zp.( * ).
+proof. by move => x y; rewrite /Zq2Zp /( * ) !inzmodK /inzmod modzMm modz_dvd 1:p_div_q. qed.
+
+lemma Zq2Zp_DM_big (F : int -> Zq) (r : int list) :
+      Zq2Zp (Rq.BasePoly.BigCf.BCA.big predT F r)
+      =
+      BCA.big predT (Zq2Zp \o F) r.
+proof.
+elim: r; first by rewrite BCA.big_nil Rq.BasePoly.BigCf.BCA.big_nil Zq2Zp0.
+move => x l @/(\o) IH; rewrite BCA.big_cons Rq.BasePoly.BigCf.BCA.big_cons {1 4}/predT /=.
+by rewrite (Zq2Zp_DM (F x) (Rq.BasePoly.BigCf.BCA.big predT F l)); congr.
+qed.
+
+lemma Zp2Zq_Zq2Zp_inv (z : Zp) : Zq2Zp (Zp2Zq z) = z.
+proof.
+rewrite /Zq2Zp /Zp2Zq inzmodK modz_small 1: ge0_asint 2:asintK //=.
+rewrite ger0_norm 2:(ltr_le_trans p _ _ (Zp.gtp_asint z)) /p /q; first smt(ge8_q).
+by apply (ler_weexpn2l 2 _ ep eq _); 2: smt(ge2_ep geep1_eq).
+qed.
+
+(* Polynomial Modular Reduction/Modulo Conversion*)
+lemma Rq2RpE (p : Rq) (i : int) : (Rq2Rp p).[i] = Zq2Zp p.[i].
+proof.
+case: (i < 0) => [lt0_i|]; first by rewrite !lt0_rcoeff // Zq2Zp0.
+move/lerNgt=> ge0_i; case: (i < n); last first.
+- by move/lerNgt=> ge_ni; rewrite !gered_rcoeff // Zq2Zp0.
+move=> lt_in; rewrite rcoeff_sum /= (BCA.bigD1 _ _ i) /=;
+              1,2: by rewrite (mem_range, range_uniq).
+rewrite rcoeffZ rcoeff_polyXn //= Zp.ZModpRing.mulr1.
+rewrite BCA.big_seq_cond BCA.big1 /=; last first.
+- by rewrite Zp.ZModpRing.addr0.
+move=> j [/mem_range rgj @/predC1 ne_ji].
+rewrite rcoeffZ rcoeff_polyXn // (eq_sym i j) ne_ji /=.
+- by rewrite Zp.ZModpRing.mulr0.
+qed.
+
+lemma Rp2RqE (p : Rp) (i : int) : (Rp2Rq p).[i] = Zp2Zq p.[i].
+proof.
+case: (i < 0) => [lt0_i|]; first by rewrite !lt0_rcoeff // Zp2Zq0.
+move/lerNgt=> ge0_i; case: (i < n); last first.
++ by move/lerNgt=> ge_ni; rewrite !gered_rcoeff // Zp2Zq0.
+move=> lt_in; rewrite rcoeff_sum /= (Rq.BasePoly.BigCf.BCA.bigD1 _ _ i) /=;
+              1,2: by rewrite (mem_range, range_uniq).
+rewrite rcoeffZ rcoeff_polyXn //= Zq.ZModpRing.mulr1.
+rewrite Rq.BasePoly.BigCf.BCA.big_seq_cond Rq.BasePoly.BigCf.BCA.big1 /=; last first.
++ by rewrite Zq.ZModpRing.addr0.
+move=> j [/mem_range rgj @/predC1 ne_ji].
+rewrite rcoeffZ rcoeff_polyXn // (eq_sym i j) ne_ji /=.
++ by rewrite Zq.ZModpRing.mulr0.
+qed.
+
+lemma Rp2RppqE (p : Rp) (i : int) : (Rp2Rppq p).[i] = Zp2Zppq p.[i].
+proof.
+case: (i < 0) => [lt0_i|]; first by rewrite !lt0_rcoeff // Zp2Zppq0.
+move/lerNgt=> ge0_i; case: (i < n); last first.
+- by move/lerNgt=> ge_ni; rewrite !gered_rcoeff // Zp2Zppq0.
+move=> lt_in; rewrite rcoeff_sum /= (Rppq.BasePoly.BigCf.BCA.bigD1 _ _ i) /=;
+              1,2: by rewrite (mem_range, range_uniq).
+rewrite rcoeffZ rcoeff_polyXn //= Zppq.ZModpRing.mulr1.
+rewrite Rppq.BasePoly.BigCf.BCA.big_seq_cond Rppq.BasePoly.BigCf.BCA.big1 /=; last first.
+- by rewrite Zppq.ZModpRing.addr0.
+move=> j [/mem_range rgj @/predC1 ne_ji].
+rewrite rcoeffZ rcoeff_polyXn // (eq_sym i j) ne_ji /=.
+- by rewrite Zppq.ZModpRing.mulr0.
+qed.
+
+lemma Rq2Rp_DM (a: Rq) (b : Rq) : morphism_2 Rq2Rp Rq.( + ) Rp.( + ).
+proof.
+move=> x y; rewrite polyXnD1_eqP => i [ge0_i ltn_i].
+by rewrite eq_sym rcoeffD !Rq2RpE rcoeffD (Zq2Zp_DM x.[i] y.[i]).
+qed.
+
+lemma Rq2Rp_MM (a: Rq) (b : Rq) : Rq2Rp (a * b) = (Rq2Rp a) * (Rq2Rp b).
+proof.
+rewrite polyXnD1_eqP => i [ge0_i ltn_i]; rewrite Rq2RpE !rcoeffM 1,2://# eq_sym. 
+have ->: 
+ (fun (i0 : int) =>
+  ((Rq2Rp a).[i0] * (Rq2Rp b).[i - i0] - (Rq2Rp a).[i0] * (Rq2Rp b).[n + i - i0]))
+ =    
+ (fun (i0 : int) =>
+  (Zq2Zp (a.[i0] * b.[i - i0] - a.[i0] * b.[n + i - i0]))).
++ rewrite fun_ext /( == ) => j. 
+  rewrite !Rq2RpE (Zq2Zp_BM (a.[j] * b.[i - j]) (a.[j] * b.[n + i - j])). 
+  by rewrite (Zq2Zp_MM a.[j] b.[i - j]) (Zq2Zp_MM a.[j] b.[n + i - j]).
+by rewrite Zq2Zp_DM_big.
+qed.
+
+lemma Rq2Rp_DotDl (a: Rq_vec) (b : Rq_vec) : Rq2Rp (dotp a b) = dotp (Rqv2Rpv a) (Rqv2Rpv b).
+proof.
+have ->:
+ dotp (Rqv2Rpv a) (Rqv2Rpv b)
+ =
+ (Big.BAdd.bigi predT (fun (i : int) => Rq2Rp (a.[i] * b.[i])) 0 l).
++ rewrite /Rqv2Rpv /dotp eq_sym /Mat_Rp.Vector."_.[_]" !offunvK /= /vclamp.
+  rewrite !Big.BAdd.big_seq &(Big.BAdd.eq_bigr) => i /= /mem_range rngi; smt(Rq2Rp_MM).
+rewrite polyXnD1_eqP => i rngi; rewrite !rcoeff_sum /= eq_sym.
+rewrite eq_sym (BCA.bigD1 _ _ i) /=; 1, 2: by rewrite (mem_range, range_uniq).
+rewrite rcoeffZ rcoeff_polyXn //= Zp.ZModpRing.mulr1.
+rewrite BCA.big_seq_cond BCA.big1 /= => [j [/mem_range rngj @/predC1 ne_ji] |].
++ by rewrite rcoeffZ rcoeff_polyXn // (eq_sym i) ne_ji /= Zp.ZModpRing.mulr0.
+rewrite Zp.ZModpRing.addr0 rcoeff_sum /=. 
+have ->: 
+ (BCA.bigi predT (fun (i0 : int) => (Rq2Rp (a.[i0] * b.[i0])).[i]) 0 l)
+ =
+ (BCA.bigi predT (fun (i0 : int) => Zq2Zp (a.[i0] * b.[i0]).[i]) 0 l).
++ by apply BCA.eq_bigr => j _ /=; rewrite Rq2RpE.
+by rewrite Zq2Zp_DM_big.   
+qed.
+
+lemma Rp2Rq_Rq2Rp_inv (p : Rp) : Rq2Rp (Rp2Rq p) = p.
+proof.
+rewrite /Rq2Rp polyXnD1_eqP => i [ge0_i ltn_i].
+rewrite rcoeff_sum /= (BCA.bigD1 _ _  i) /=; 1, 2: by rewrite (mem_range, range_uniq).
+rewrite rcoeffZ rcoeff_polyXn //= Rp2RqE Zp2Zq_Zq2Zp_inv Zp.ZModpRing.mulr1.
+rewrite BCA.big_seq_cond BCA.big1 /=; last by rewrite Zp.ZModpRing.addr0.
+move => j [/mem_range rgj @/predC1 ne_ji].
+by rewrite rcoeffZ rcoeff_polyXn // (eq_sym i j) ne_ji Zp.ZModpRing.mulr0 //.
+qed.
+
+(* Polynomial Vector Modular Reduction/Modulo Conversion *)
+lemma Rpv2RqvE (p : Rp_vec) (i : int) : (Rpv2Rqv p).[i] = Rp2Rq p.[i].
+proof.
+rewrite /Rpv2Rqv /Mat_Rq.Vector."_.[_]" offunvK /vclamp.
+case (0 <= i && i < l) => //; move/(Mat_Rp.Vector.getv_out p i) => ->.
+rewrite /Rp2Rq eq_sym BigRq.XnD1CA.big_seq BigRq.XnD1CA.big1 => //= j /mem_range [ge0_j ltn_j].
+by rewrite rcoeff0 Zp2Zq0 scale0p.
+qed.
+
+lemma Rqv2RpvE (p : Rq_vec) (i : int) : (Rqv2Rpv p).[i] = Rq2Rp p.[i].
+proof.
+rewrite /Rqv2Rpv /Mat_Rp.Vector."_.[_]" offunvK /vclamp.
+case (0 <= i && i < l) => //; move/(Mat_Rq.Vector.getv_out p i) => ->.
+rewrite /Rq2Rp eq_sym BigRp.XnD1CA.big_seq BigRp.XnD1CA.big1 => //= j; case/mem_range => ge0_j ltn_j.
+have ->: Zq2Zp Rq.zeroXnD1.[j] = Zp.zero; 2: rewrite /( ** ) scale0p //.
+by rewrite /zeror /"_.[_]" piK 1:reducedP 1:degC // -/Rq.BasePoly."_.[_]" poly0E /Zq2Zp Zq.zeroE.
+qed.
+
+lemma Rpv2Rqv_Rqv2Rpv_inv (pv : Rp_vec) : Rqv2Rpv (Rpv2Rqv pv) = pv.
+proof.
+rewrite /Rqv2Rpv eq_vectorP => i rngi.
+by rewrite {1}/Mat_Rp.Vector."_.[_]" offunvK /vclamp rngi /= Rpv2RqvE Rp2Rq_Rq2Rp_inv.
+qed.
+
+(* - Distribution Mapping - *)
+lemma duni_Zq2Zp : dmap DZqP.dunifin Zq2Zp = DZpP.dunifin.
 proof.
 rewrite !(DZqP.dzmodE, DZpP.dzmodE) dmap_comp.
 have ->: Zq2Zp \o Zq.inzmod = Zp.inzmod.
@@ -348,29 +592,9 @@ rewrite -dmap1E; apply/eq_distr/duni_range_dvd/p_div_q.
 - by apply/(ltr_le_trans 4)/ge4_p.
 qed.
 
-op Rq2Rp (p : Rq) : Rp =
-  BigRp.XnD1CA.bigi predT (fun (i : int) => Zq2Zp p.[i] ** exp Rp.iX i) 0 n.
-
-op Rqv2Rpv (p : Rq_vec) : Rp_vec = offunv (fun (i : int) => Rq2Rp p.[i]).
-
-lemma Rq2RpE (p : Rq) (i : int) : (Rq2Rp p).[i] = Zq2Zp p.[i].
+lemma dRq2dRp : dmap dRq Rq2Rp = dRp.
 proof.
-case: (i < 0) => [lt0_i|]; first by rewrite !lt0_rcoeff // Zq2Zp0.
-move/lerNgt=> ge0_i; case: (i < n); last first.
-- by move/lerNgt=> ge_ni; rewrite !gered_rcoeff // Zq2Zp0.
-move=> lt_in; rewrite rcoeff_sum /= (BCA.bigD1 _ _ i) /=;
-  1,2: by rewrite (mem_range, range_uniq).
-rewrite rcoeffZ rcoeff_polyXn //= Zp.ZModpRing.mulr1.
-rewrite BCA.big_seq_cond BCA.big1 /=; last first.
-- by rewrite Zp.ZModpRing.addr0.
-move=> j [/mem_range rgj @/predC1 ne_ji].
-rewrite rcoeffZ rcoeff_polyXn // (eq_sym i j) ne_ji /=.
-- by rewrite Zp.ZModpRing.mulr0.
-qed.
-
-lemma duni_Rp_Rq : dmap Rq.dpolyXnD1 Rq2Rp = Rp.dpolyXnD1.
-proof.
-rewrite /Rq.dpolyXnD1 /Rp.dpolyXnD1 -duni_Zp_Zq.
+rewrite /dRq /dRp /Rq.dpolyXnD1 /Rp.dpolyXnD1 -duni_Zq2Zp.
 rewrite !(dmap_comp, dlist_dmap) &(eq_dmap_in).
 move=> xs /(supp_dlist_size _ _ _ ge0_n) => szxs @/(\o).
 apply/Rp.polyXnD1_eqP=> i rgi; rewrite Rq2RpE.
@@ -378,484 +602,26 @@ rewrite !piK; ~-1: by rewrite (reduced_polyL) ?size_map szxs.
 by rewrite !polyLE (nth_map Zq.zero) ?szxs.
 qed.
 
-lemma Rqv2RpvE (p : Rq_vec) (i : int) : (Rqv2Rpv p).[i] = Rq2Rp p.[i].
+lemma dRqv2dRpv: dmap dRq_vec Rqv2Rpv = dRp_vec.
 proof.
-  rewrite /Rqv2Rpv /Mat_Rp.Vector."_.[_]" offunvK /vclamp.
-  case (0 <= i && i < l) => //; move/(Mat_Rq.Vector.getv_out p i) => ->.
-  rewrite /Rq2Rp eq_sym BigRp.XnD1CA.big_seq BigRp.XnD1CA.big1 => //= j; 
-          case/mem_range => ge0_j ltn_j.
-  have ->: Zq2Zp Rq.zeroXnD1.[j] = Zp.zero; 2: rewrite /( ** ) scale0p //.
-  by rewrite /zeror /"_.[_]" piK 1:reducedP 1:degC // 
-     -/Rq.BasePoly."_.[_]" poly0E /Zq2Zp Zq.zeroE.
+rewrite /dRp_vec /dRp /dRq_vec /dRq /Rq.dpolyXnD1 /Rp.dpolyXnD1 /dvector -duni_Zq2Zp.
+rewrite !(dmap_comp, dlist_dmap, -djoin_dmap_nseq) /(\o).
+apply eq_dmap_in => x /supp_djoin [sxl /allP] /= xele.
+rewrite size_nseq maxrE lezNgt -(lez_add1r _ l) ge1_l /= in sxl.
+apply eq_vectorP => i [ge0_i ltl_i]; rewrite Rqv2RpvE /"_.[_]" !offunvK /vclamp ge0_i ltl_i /=.
+rewrite !(nth_map witness) /=; 1, 2: smt().
+have sxn : size (nth witness x i) = n.
++ move: (xele ((dlist DZqP.dunifin n), (nth witness x i)) _) => /=.
+  - by rewrite sxl &(mem_zip_nseqL) mem_nth //#.
+  - by apply supp_dlist_size. 
+apply Rp.polyXnD1_eqP => j [gt0_j ltn_j]; rewrite Rq2RpE. 
+rewrite !piK; first 2 by rewrite reduced_polyL ?size_map lez_eqVlt; left. 
+by rewrite !polyLE (nth_map Zq.zero) //#.
 qed.
 
-lemma duni_Rp_Rq_vec: dmap dRq_vec Rqv2Rpv = dRp_vec.
-proof.
-  rewrite /dRp_vec /dRp /dRq_vec /dRq /Rq.dpolyXnD1 /Rp.dpolyXnD1 /dvector -duni_Zp_Zq.
-  rewrite !(dmap_comp, dlist_dmap, -djoin_dmap_nseq) /(\o).
-  apply eq_dmap_in => x /supp_djoin [sxl /allP] /= xele.
-  rewrite size_nseq maxrE lezNgt -(lez_add1r _ l) ge1_l /= in sxl.
-  apply eq_vectorP => i [ge0_i ltl_i]; rewrite Rqv2RpvE /"_.[_]" !offunvK /vclamp ge0_i ltl_i /=.
-  rewrite !(nth_map witness) /=; 1, 2: smt().
-  have sxn : size (nth witness x i) = n.
-  + move: (xele ((dlist DZqP.dunifin n), (nth witness x i)) _) => /=.
-    - by rewrite sxl &(mem_zip_nseqL) mem_nth //#.
-    - by apply supp_dlist_size. 
-  apply Rp.polyXnD1_eqP => j [gt0_j ltn_j]; rewrite Rq2RpE. 
-  rewrite !piK; first 2 by rewrite reduced_polyL ?size_map lez_eqVlt; left. 
-  by rewrite !polyLE (nth_map Zq.zero) //#.
-qed.
-
-(* - Constants - *)
-const h1 : Rq = pi (to_polyd (fun _ => Zq.inzmod (2 ^ (eq - ep - 1)))).
-const h2 : Rq = pi (to_polyd (fun _ => Zq.inzmod (2 ^ (ep - 2) - 2 ^ (ep - et - 2)))).
-const h : Rq_vec = vectc h1.
-
-(* -- Cryptographic Types and Distributions  -- *)
-type seed.
-type pkey.
-type skey.
-type plaintext.
-type ciphertext.
-
-op [lossless full uniform] dseed : seed distr.
-
-(* -- Operations -- *)
-op gen : seed -> Rq_mat.
-
-op shl (x : int, ex : int) : int = x * 2 ^ ex.
-op shl_enc (x : R2, ex : int) : Rp = pi (to_polyd (fun i => Zp.inzmod (shl (Z2.asint x.[i]) ex))).
-op shl_dec (x : R2t) : Rp = pi (to_polyd (fun i => Zp.inzmod (shl (Z2t.asint x.[i]) (ep - et - 1)))).
-
-op shr (x : int, ex : int) : int = x %/ 2 ^ ex.
-
-op scale (x : int, ea : int, eb : int) : int = shr x (ea - eb).
-
-op scale_Zq_Zp (x : Zq) : Zp = Zp.inzmod (scale (Zq.asint x) eq ep).
-op scale_Zp_Z2t (x : Zp) : Z2t = Z2t.inzmod (scale (Zp.asint x) ep (et + 1)).
-op scale_Zp_Z2 (x : Zp) : Z2 = Z2.inzmod (scale (Zp.asint x) ep 1).
-op scale_Zp_Zppq (x : Zp) : Zppq = Zppq.inzmod (scale (Zp.asint x) ep (2 * ep - eq)).
-op scale_Zp_Zp (x : Zp) : Zp = Zp.inzmod (scale (Zp.asint x) ep ep).
-op scale_Zppq_Z2t (x : Zppq) : Z2t = Z2t.inzmod (scale (Zppq.asint x) (2 * ep - eq) (et + 1)).
-
-op scale_Rq_Rp (x : Rq) : Rp = pi (to_polyd (fun i => scale_Zq_Zp x.[i])).
-op scale_Rp_R2t (x : Rp) : R2t = pi (to_polyd (fun i => scale_Zp_Z2t x.[i])).
-op scale_Rp_R2 (x : Rp) : R2 = pi (to_polyd (fun i => scale_Zp_Z2 x.[i])).
-op scale_Rp_Rppq (x : Rp) : Rppq = pi (to_polyd (fun i => scale_Zp_Zppq x.[i])).
-op scale_Rp_Rp (x : Rp) : Rp = pi (to_polyd (fun i => scale_Zp_Zp x.[i])).
-op scale_Rppq_R2t (x : Rppq) : R2t = pi (to_polyd (fun i => scale_Zppq_Z2t x.[i])).
-
-op scale_vec_Rq_Rp (v : Rq_vec) : Rp_vec = offunv (fun i => scale_Rq_Rp v.[i]).
-
-op mod_p_Rq (x : Rq) : Rp = pi (to_polyd (fun i => Zp.inzmod (Zq.asint x.[i]))).
-op mod_p_Rq_vec (v : Rq_vec) : Rp_vec = offunv (fun i => mod_p_Rq v.[i]).
-
-op mod_q_Rp (x : Rp) : Rq = pi (to_polyd (fun i => Zq.inzmod (Zp.asint x.[i]))).
-op mod_q_Rp_vec (v : Rp_vec) : Rq_vec = offunv (fun i => mod_q_Rp v.[i]).
-
-op mod_ppq_Rp (x : Rp) : Rppq =  pi (to_polyd (fun i => Zppq.inzmod (Zp.asint x.[i]))).
-
-op pk_encode ['a] : 'a -> pkey.
-op pk_decode ['a] : pkey -> 'a.
-
-op sk_encode ['a] : 'a -> skey.
-op sk_decode ['a] : skey -> 'a.
-
-op m_encode ['a] : 'a -> plaintext.
-op m_decode ['a] : plaintext -> 'a.
-
-op c_encode ['a] : 'a -> ciphertext.
-op c_decode ['a] : ciphertext -> 'a.
-
-(* - Properties  - *)
-axiom pk_enc_dec_inv ['a] (x : 'a) : pk_decode (pk_encode x) = x. 
-axiom sk_enc_dec_inv ['a] (x : 'a) : sk_decode (sk_encode x) = x. 
-axiom m_enc_dec_inv ['a] (x : 'a) : m_decode (m_encode x) = x. 
-axiom c_enc_dec_inv ['a] (x : 'a) : c_decode (c_encode x) = x. 
-
-lemma scale_comp (x ea eab eb : int):
-      0 <= x => 0 <= eb => eb <= eab => eab <= ea =>
-      scale x ea eb = scale (scale x ea eab) eab eb. 
-proof. 
-  (* Context *)
-  move=> ge0_x ge0_eb geeb_eab geeab_ea; rewrite /scale /shr. 
-  move: (divz_eq x (2^(ea - eb))) 
-        (divz_eq x (2^(ea - eab))) 
-        (divz_eq (x %/ 2 ^ (ea - eab)) (2^(eab - eb))).
-  pose dmain := 2 ^ (ea - eb); pose d0 := 2 ^ (ea - eab); pose d1 := 2 ^ (eab - eb).
-  pose qmain := x %/ dmain; pose q0 := x %/ d0; pose q1 := x %/ d1.
-  pose rmain := x %% dmain; pose r0 := x %% d0; pose r1 := x %% d1.
-  move=> divmain div0 div1.
-  
-  have gt0_d0: 0 < d0.
-  + by apply expr_gt0.
-  have gt0_d1: 0 < d1.
-  + by apply expr_gt0.
-
-  have eq_dmain_d0d1: dmain = d0 * d1.
-  + rewrite /dmain /d0 /d1 -exprD_nneg. 
-    - by rewrite -(lez_add2r eab 0 (ea - eab)) -addrA /= geeab_ea.
-    - by rewrite -(lez_add2r eb 0 (eab - eb)) -addrA /= geeb_eab.
-    - by congr; rewrite -addzA addKz.
-
-  (* Main Proof *)
-  move: (euclideU dmain qmain (q0 %/ d1) rmain (q0 %% d1 * d0 + r0)).
-  + have <-: x = q0 %/ d1 * dmain + (q0 %% d1 * d0 + r0).
-    - by rewrite eq_dmain_d0d1 (mulzC d0 d1) -(mulzA (q0 %/ d1)) addzA -(mulzDl _ _ d0) -div1.
-  rewrite -divmain /=.  
-  + have -> /=: 0 <= rmain && rmain < `| dmain |.
-    - split; [by apply /modn_ge0 /ge0_x | move => ge0_rmain].
-      * by rewrite ltz_mod neq_ltz; right; apply expr_gt0.
-  + have -> /=:  0 <= q0 %% d1 * d0 + r0 && q0 %% d1 * d0 + r0 < `| dmain |.
-    - split; 1: by apply /addz_ge0 /modn_ge0 /ge0_x /mulr_ge0 /ltzW /gt0_d0 /modz_ge0 /neq_ltz; right.
-      * rewrite ger0_norm eq_dmain_d0d1; first by rewrite mulr_ge0 ltzW.
-        rewrite (ltr_le_trans ((d1 - 1) * d0 + d0) _ (d0 * d1)) 3://.
-        + apply (ler_lt_add _ _ r0 d0); last by apply ltz_pmod.
-          apply /(ler_pmul _ _ d0 d0) /lezz; [by apply /modz_ge0 /neq_ltz; right | by apply ltzW |].
-          by apply (lez_add2l 1); rewrite lez_add1r -addzCA /= ltz_pmod.
-        + by rewrite mulzDl mulNr /= -addzA addNz /= mulzC; apply lezz.
-   by case.
-qed.
-
-lemma ispoly_fun_scale_Zq_Zp (x : Rq) : ispoly (fun i => scale_Zq_Zp x.[i]).
-proof.
-  split; [| exists (deg (crepr x) - 1)] => [c lt0_c | c gtdeg1_c] /=;
-         rewrite /scale_Zq_Zp /scale /shr; have ->: asint x.[c] = 0; 
-         2, 4: by rewrite div0z -Zp.zeroE asintK. 
-  + by rewrite lt0_coeff 2:-Zq.zeroE.
-  + by rewrite gedeg_coeff 2:-Zq.zeroE; rewrite -lez_add1r addzC /= in gtdeg1_c.
-qed.
-
-lemma ispoly_fun_scale_Zp_Zppq (x : Rp) : ispoly (fun i => scale_Zp_Zppq x.[i]).
-proof.
-  split; [| exists (deg (crepr x) - 1)] => [c lt0_c | c gtdeg1_c] /=;
-         rewrite /scale_Zp_Zppq /scale /shr; have ->: asint x.[c] = 0; 
-         2, 4: by rewrite div0z -Zppq.zeroE asintK. 
-  + by rewrite lt0_coeff 2:-Zp.zeroE.
-  + by rewrite gedeg_coeff 2:-Zp.zeroE; rewrite -lez_add1r addzC /= in gtdeg1_c.
-qed.
-
-lemma ispoly_fun_scale_Zp_Zp (x : Rp) : ispoly (fun i => scale_Zp_Zp x.[i]).
-proof.
-  split; [| exists (deg (crepr x) - 1)] => [c lt0_c | c gtdeg1_c] /=;
-         rewrite /scale_Zp_Zp /scale /shr; have ->: asint x.[c] = 0; 
-         2, 4: by rewrite div0z -Zp.zeroE asintK. 
-  + by rewrite lt0_coeff 2:-Zp.zeroE.
-  + by rewrite gedeg_coeff 2:-Zp.zeroE; rewrite -lez_add1r addzC /= in gtdeg1_c.
-qed.
-
-lemma reduced_topolyd_scale_Zq_Zp (x : Rq): 
-      reduced (to_polyd (fun i => scale_Zq_Zp x.[i])).
-proof.
-  rewrite reducedP deg_leP 1:ge0_n => i gen_i; rewrite coeffE 2:/= 1:ispoly_fun_scale_Zq_Zp.
-  rewrite /scale_Zq_Zp /scale /shr; have ->: asint x.[i] = 0; 2: by rewrite div0z -Zp.zeroE asintK.
-  by rewrite -Zq.zeroE Zq.asint_eq gedeg_coeff 1:(lez_trans n) /crepr 1:deg_reduce.
-qed.
-
-lemma reduced_topolyd_scale_Zp_Zppq (x : Rp): 
-      reduced (to_polyd (fun i => scale_Zp_Zppq x.[i])).
-proof.
-  rewrite reducedP deg_leP 1:ge0_n => i gen_i; rewrite coeffE 2:/= 1:ispoly_fun_scale_Zp_Zppq.
-  rewrite /scale_Zp_Zppq /scale /shr; have ->: asint x.[i] = 0; 2: by rewrite div0z -Zppq.zeroE asintK.
-  by rewrite -Zp.zeroE Zp.asint_eq gedeg_coeff 1:(lez_trans n) /crepr 1:deg_reduce.
-qed.
-
-lemma scale_comp_Zp_Zppq_Z2t (x : Zp):
-      scale_Zp_Z2t x = scale_Zppq_Z2t (scale_Zp_Zppq x).
-proof. 
-  rewrite /scale_Zp_Z2t /scale_Zppq_Z2t /scale_Zp_Zppq Zppq.inzmodK -Z2t.eq_inzmod; do 2! congr.
-  have ge2epeq_ep: 2 * ep - eq <= ep.
-  + by rewrite mulzC -intmulz mulr2z -(lez_add2l (-ep)) -addzA addzCA addzA /= 
-               subz_le0 (lez_trans (ep + 1)); [rewrite (lez_addl _ 1) | apply geep1_eq].
-  rewrite (modz_small (scale (Zp.asint x) ep (2 * ep - eq)) (p * p %/ q)); first split; 
-          rewrite /scale /shr => [| ?].
-  + by apply /divz_ge0 /Zp.ge0_asint /expr_gt0.
-  + rewrite ger0_norm; first by apply /(lez_trans 2) /ge2_ppq. 
-    apply ltz_divLR; first by apply expr_gt0. 
-    rewrite -eq_22epeq_ppq -exprD_nneg; first by rewrite subz_ge0 (lez_trans (eq + 1)); 
-            [rewrite (lez_addl _ 1) | apply geeq1_2ep].
-    - by rewrite subz_ge0.
-    - by rewrite mulzC -intmulz mulr2z addzCA /= (ltr_le_trans p) 2:lezz Zp.gtp_asint.
-  apply /(scale_comp (Zp.asint x)) /ge2epeq_ep; 
-        [apply Zp.ge0_asint | by apply /(lez_trans 1) /ge1_et1 |].
-  rewrite mulzC -intmulz mulr2z -(lez_add2r (-(et + 1))) /= -(lez_add2l (eq)) addzAC addzCA /= 
-          -(lez_add2r (-ep)) addzAC (IntID.subrK ep (-ep)) opprD addzA.
-  by apply sec_assumption.
-qed.
-
-lemma scale_comp_Rp_Rppq_R2t (x : Rp):
-      scale_Rp_R2t x = scale_Rppq_R2t (scale_Rp_Rppq x).
-proof.
-  rewrite /scale_Rp_R2t /scale_Rppq_R2t /scale_Rp_Rppq; do 2! congr; rewrite fun_ext /(==) => i. 
-  by rewrite piK 1:reduced_topolyd_scale_Zp_Zppq coeffE 
-             1:ispoly_fun_scale_Zp_Zppq /= scale_comp_Zp_Zppq_Z2t.
-qed.
-
+(* Scaling *)
 lemma scale_id (x ea eb : int) : ea = eb => scale x ea eb = x.
 proof. by move=> eq_eaeb; rewrite /scale /shr eq_eaeb addzN expr0. qed.
-
-lemma scale_Zp_Zp_id (x : Zp) : scale_Zp_Zp x = x.
-proof. by rewrite /scale_Zp_Zp scale_id 2: Zp.asintK. qed.
-
-lemma scale_Rp_Rp_id (x : Rp) : scale_Rp_Rp x = x.
-proof. 
-  rewrite /scale_Rp_Rp -{2}creprK; congr.
-  rewrite poly_eqP => c ge0_c; rewrite coeffE /= 1:ispoly_fun_scale_Zp_Zp &(scale_Zp_Zp_id). 
-qed.
-
-lemma mod_p_Zq_h1_id : 
-      Zp.asint (Zp.inzmod (2 ^ (eq - ep - 1))) 
-      = 
-      Zq.asint (Zq.inzmod (2 ^ (eq - ep - 1))).
-proof.
-  rewrite Zp.inzmodK Zq.inzmodK ?modz_small /p /q //; first 2 split => [| ?];
-          [by apply expr_ge0 |
-           rewrite ger0_norm ?expr_ge0 // ltz_def ler_weexpn2l // ?andbT; first split => [| ?]; 
-           1: rewrite -(lez_add2r 1) /= -(lez_add2r ep) -addzA addzC /= geep1_eq].
-  + by rewrite -(lez_add2r ep) addzAC addzC -addzA addzC -mulr2z intmulz mulzC (lez_trans (eq + 1)) 
-           1:-(lez_add2r 1) /= 1:lez_addl // geeq1_2ep.
-  + move: (ieexprIn 2 _ _ ep (eq - ep - 1) (lez_trans 2 0 ep _ ge2_ep) _) => //.
-    - by rewrite -(lez_add2r 1) /= -(lez_add2r ep) -addzA /= addzC geep1_eq.   
-    move /contra; apply; rewrite neq_ltz; right.
-    by rewrite -(ltz_add2l ep) /= addzCA addzC addzA addzC 2!addzA addzC /= -mulr2z intmulz mulzC 
-                (ltr_le_trans (eq + 1)) 1: ltz_add2l 2: geeq1_2ep.
-  + by rewrite -(lez_add2l (-eq)) 2!addzA /= -(lez_add2l ep) addzA /= (lez_trans 2) // ge2_ep.
-  + move: (ieexprIn 2 _ _ eq (eq - ep - 1) (lez_trans 3 0 eq _ ge3_eq) _) => //.
-    - by rewrite -(lez_add2r 1) /= -(lez_add2r ep) -addzA /= addzC geep1_eq.
-    move /(contra); apply; rewrite neq_ltz; right.
-   by rewrite -(ltz_add2l (-eq)) 2!addzA /= -(ltz_add2l ep) addzA /= (ltr_le_trans 2) 2:ge2_ep.
-qed.
-
-lemma eq_scaleZqZp_modZppq_scaleZpZppq (x : Zq) (m : Z2) :
-      Zppq.inzmod (Zp.asint ((scale_Zq_Zp x) + (Zp.inzmod (shl (Z2.asint m) (2 * ep - eq - 1)))))
-      =
-      scale_Zp_Zppq ((Zp.inzmod (Zq.asint x)) + Zp.inzmod (shl (Z2.asint m) (ep - 1))).
-proof.
-  rewrite /scale_Zq_Zp /scale_Zp_Zppq /scale /shr /shl !Zp.inzmodK !modzDm 
-          {2}(mulzC 2) -(intmulz ep) mulr2z !opprD !addzA /= (addzC _ eq).
-  have ge0_eqep: 0 <= eq - ep; 1: by apply /(lez_trans 1) /(lez_add2l ep); 
-       2: rewrite addzCA /= geep1_eq.
-  have leep_eq_ep: eq - ep <= ep; 1: by rewrite -(lez_add2r ep) -addzA /= -mulr2z intmulz mulzC 
-                                                 (lez_trans (eq + 1)) 2:geeq1_2ep lez_addl.
-  have ge0_2epeq: 0 <= 2 * ep - eq; 1: by rewrite -(lez_add2r eq) -addzA /= (lez_trans (eq + 1)) 
-                                                  2:geeq1_2ep lez_addl.
-  have leep_2epeq: 2 * ep - eq <= ep; first rewrite mulzC -intmulz mulr2z -(lez_add2l (-ep)) 2!addzA;
-       move: (oppz_le0 (eq - ep)); rewrite ge0_eqep opprD /= addzC => -> //.
-  case: (Z2.asint m = 0) => [-> /= | /neq_ltz]; last case => [lt0_m | gt0_m]; 
-        move: (Z2.Sub.valP m) => [ge0_m lt2_m].
-  + by rewrite -Zppq.eq_inzmod -eq_22epeq_ppq /p /q (modz_pow2_div); 
-               [apply Zq.ge0_asint | 
-                split | 
-                rewrite opprD (addzC _ ep) addzA -mulr2z intmulz (mulzC ep) modz_mod modz_dvd_pow].
-  + by rewrite -/Z2.asint lezNgt in ge0_m.
-  have -> /= {gt0_m ge0_m lt2_m}: Z2.asint m = 1; first rewrite eqz_leq; split. 
-  + by rewrite -/Z2.asint -lez_add1r -(lez_add2l (-1)) /= in lt2_m.
-  + by rewrite -lez_add1r in gt0_m.
-  rewrite -Zppq.eq_inzmod -eq_22epeq_ppq /p modz_dvd_pow; 1: by split.
-  rewrite modz_pow2_div; [by apply /addz_ge0 /expr_ge0; 1: apply Zq.ge0_asint | by split |]. 
-  rewrite opprD (addzC (-eq)) addzA /= -mulr2z intmulz (mulzC ep) modz_mod divzDr 1: dvdz_exp2l. 
-  + by split => [| ?]; last rewrite -(lez_add2r 1) -(lez_add2l ep) -!addzA /= !addzA addzAC 
-                                     addzC !addzA /= -mulr2z intmulz mulzC geeq1_2ep.
-  have -> //: 2 ^ (ep - 1) %/ 2 ^ (eq - ep) = 2 ^ (2 * ep - eq - 1).
-  rewrite eq_sym eqz_div 2:dvdz_exp2l 3: -exprD_nneg; last congr; rewrite //#. 
-  + by rewrite neq_ltz; right; apply expr_gt0.
-  + by split => [| ?]; last rewrite -(lez_add2r 1) -(lez_add2l ep) -!addzA /= !addzA 
-                                     addzAC addzC !addzA /= -mulr2z intmulz mulzC geeq1_2ep.
-  + by rewrite -(lez_add2r 1) -addzA /= -(lez_add2r eq) -addzA addzC /= geeq1_2ep.
-  + by apply /(lez_trans 1) /(lez_add2l ep); 2: rewrite addzCA /= geep1_eq.
-qed. 
-
-lemma eq_scaleRqRp_modRppq_scale_Rppq (x : Rq) (m : R2) :
-      mod_ppq_Rp ((scale_Rq_Rp x) + (shl_enc m (2 * ep - eq - 1)))
-      =
-      scale_Rp_Rppq ((mod_p_Rq x) + (shl_enc m (ep - 1))).
-proof.
-  (* Re-occuring Goals *)
-  have ispoly_shlm_pp2q: 
-       ispoly (fun (i0 : int) => (Zp.inzmod (shl (Z2.asint m.[i0]) (2 * ep - eq - 1)))).
-  + split; [| exists (deg (crepr m) - 1)] => [c lt0_c | c gtdeg1_c] /=; have ->: asint m.[c] = 0;
-           2, 4: rewrite /shl mul0r //; 1, 2: rewrite -Z2.zeroE asint_eq. 
-    - by apply R2.BasePoly.lt0_coeff. 
-    - by apply R2.BasePoly.gedeg_coeff; rewrite -lez_add1r addzC /= in gtdeg1_c. 
-
-  have ispoly_xmodp : ispoly (fun (i0 : int) => (Zp.inzmod (Zq.asint x.[i0]))).
-  + split; [| exists (deg (crepr x) - 1)] => [c lt0_c | c gtdeg1_c] /=; have ->: asint x.[c] = 0;
-           rewrite // -Zq.zeroE asint_eq.
-    - by apply Rq.BasePoly.lt0_coeff.
-    - by apply Rq.BasePoly.gedeg_coeff; rewrite -lez_add1r addzC /= in gtdeg1_c.
-
-  have ispoly_shlm_p2 : ispoly (fun (i0 : int) => (Zp.inzmod (shl (Z2.asint m.[i0]) (ep - 1)))).
-  + split; [| exists (deg (crepr m) - 1)] => [c lt0_c | c gtdeg1_c] /=; have ->: asint m.[c] = 0;
-           2, 4: rewrite /shl mul0r //; 1, 2: rewrite -Z2.zeroE asint_eq. 
-    - by apply R2.BasePoly.lt0_coeff. 
-    - by apply R2.BasePoly.gedeg_coeff; rewrite -lez_add1r addzC /= in gtdeg1_c.
-
-  (* Main Proof *)
-  rewrite /mod_ppq_Rp /scale_Rp_Rppq; do 2! congr; rewrite fun_ext /(==) => i.
-  rewrite /mod_p_Rq /scale_Rq_Rp /shl_enc !addE !piK; 1, 2: apply Rp.reducedD;
-          2, 3, 4: rewrite reducedP deg_leP 1:ge0_n => j gen_j; 2, 3, 4: rewrite coeffE /=.
-  + by apply reduced_topolyd_scale_Zq_Zp.
-  + by apply ispoly_shlm_pp2q.
-  + have ->: asint m.[j] = 0; 2: rewrite /shl mul0r //.
-    - by rewrite -Z2.zeroE asint_eq gedeg_coeff 1:(lez_trans n) 1:&(R2.deg_crepr).
-  + by apply ispoly_xmodp.
-  + by have ->: asint x.[j] = 0; rewrite // -Zq.zeroE asint_eq gedeg_coeff // 
-                                         (lez_trans n) ?deg_crepr.
-  + by apply ispoly_shlm_p2.
-  + have ->: asint m.[j] = 0; 2: rewrite /shl mul0r //.
-    - by rewrite -Z2.zeroE asint_eq gedeg_coeff 1:(lez_trans n) 1:&(R2.deg_crepr).
-  rewrite !polyDE !coeffE.
-  + by apply ispoly_fun_scale_Zq_Zp.
-  + by apply ispoly_shlm_pp2q.
-  + by apply ispoly_xmodp.
-  + by apply ispoly_shlm_p2.
-  by apply eq_scaleZqZp_modZppq_scaleZpZppq.
-qed.
-
-pragma Goals:printall.
-
-lemma Zq2Zp_DDl (a b : Zq) : Zq2Zp (a + b) = Zq2Zp a + Zq2Zp b.
-proof. by rewrite /Zq2Zp /( + ) !inzmodK /inzmod modzDm modz_dvd 1:p_div_q. qed.
-
-lemma Zq2Zp_BDl (a b : Zq) : Zq2Zp (a - b) = Zq2Zp a - Zq2Zp b.
-proof. 
-by rewrite /Zq2Zp /( + ) !inzmodK modzNm /inzmod modzDm modzDmr modz_dvd 1:p_div_q. 
-qed.
-
-lemma Zq2Zp_MDl (a b : Zq) : Zq2Zp (a * b) = Zq2Zp a * Zq2Zp b.
-proof. by rewrite /Zq2Zp /( * ) !inzmodK /inzmod modzMm modz_dvd 1:p_div_q. qed.
-
-lemma Rq2Rp_DDl (a: Rq) (b : Rq) :
-      Rq2Rp (a + b) = (Rq2Rp a) + (Rq2Rp b).
-proof.
-by rewrite polyXnD1_eqP => i [ge0_i ltn_i]; rewrite eq_sym rcoeffD !Rq2RpE rcoeffD Zq2Zp_DDl.
-qed.
-
-lemma Rq2Rp_MDl (a: Rq) (b : Rq) :
-      Rq2Rp (a * b) = (Rq2Rp a) * (Rq2Rp b).
-proof.
-rewrite polyXnD1_eqP => i [ge0_i ltn_i]; rewrite Rq2RpE !rcoeffM 1,2://# eq_sym. 
-have ->: 
- (fun (i0 : int) =>
-  ((Rq2Rp a).[i0] * (Rq2Rp b).[i - i0] - (Rq2Rp a).[i0] * (Rq2Rp b).[n + i - i0]))
- =    
- (fun (i0 : int) =>
-  (Zq2Zp (a.[i0] * b.[i - i0] - a.[i0] * b.[n + i - i0]))).
-+ by rewrite fun_ext /( == ) => j; rewrite !Rq2RpE Zq2Zp_BDl !Zq2Zp_MDl.
-admit.
-qed.
-
-lemma Rq2Rp_DotDl (a: Rq_vec) (b : Rq_vec) :
-      Rq2Rp (dotp a b) = dotp (Rqv2Rpv a) (Rqv2Rpv b).
-proof.
-rewrite /Rqv2Rpv /dotp eq_sym.
-rewrite /Mat_Rp.Vector."_.[_]" !offunvK /= /vclamp.
-have ->:
-(Big.BAdd.bigi predT
-   (fun (i : int) =>
-      (if 0 <= i && i < l then Rq2Rp (a.[i]) else Rp.zeroXnD1) *
-      if 0 <= i && i < l then Rq2Rp (b.[i]) else Rp.zeroXnD1) 0 l)
-=
-(Big.BAdd.bigi predT
-   (fun (i : int) =>
-      Rq2Rp (a.[i] * b.[i])) 0 l).
-rewrite !Big.BAdd.big_seq &(Big.BAdd.eq_bigr) => i /= /mem_range [ge0_i ltl_i]; smt(Rq2Rp_MDl).
-rewrite polyXnD1_eqP => i rngi. 
-rewrite !rcoeff_sum /= eq_sym.
-rewrite (BCA.bigD1 _ _ i) /=;  1, 2: by rewrite (mem_range, range_uniq).
-rewrite rcoeffZ rcoeff_polyXn //= Zp.ZModpRing.mulr1.
-rewrite BCA.big_seq_cond BCA.big1 /= => [j [/mem_range rngj @/predC1 ne_ji] |].
-+ by rewrite rcoeffZ rcoeff_polyXn // (eq_sym i) ne_ji /= Zp.ZModpRing.mulr0.
-rewrite Zp.ZModpRing.addr0 rcoeff_sum /=. 
-have ->: 
-(BCA.bigi predT (fun (i0 : int) => (Rq2Rp (a.[i0] * b.[i0])).[i]) 0 l)
-=
-(BCA.bigi predT (fun (i0 : int) => Zq2Zp (a.[i0] * b.[i0]).[i]) 0 l).
-+ by apply BCA.eq_bigr => j _ /=; rewrite Rq2RpE.   
-admit.
-qed.
-
-op Zp2Zq (z : Zp) : Zq = Zq.inzmod (Zp.asint z).
-
-op Rp2Rq (p : Rp) : Rq =
-  BigRq.XnD1CA.bigi predT (fun (i : int) => Zp2Zq p.[i] ** exp Rq.iX i) 0 n.
-
-op Rpv2Rqv (pv : Rp_vec) : Rq_vec = offunv (fun (i : int) => Rp2Rq pv.[i]).
-
-lemma Zp2Zq0 : Zp2Zq Zp.zero = Zq.zero.
-proof. by rewrite -eq_inzmod zeroE mod0z. qed.
-
-lemma Rp2RqE (p : Rp) (i : int) : (Rp2Rq p).[i] = Zp2Zq p.[i].
-proof.
-case: (i < 0) => [lt0_i|]; first by rewrite !lt0_rcoeff // Zp2Zq0.
-move/lerNgt=> ge0_i; case: (i < n); last first.
-+ by move/lerNgt=> ge_ni; rewrite !gered_rcoeff // Zp2Zq0.
-move=> lt_in; rewrite rcoeff_sum /= (Rq.BasePoly.BigCf.BCA.bigD1 _ _ i) /=;
-              1,2: by rewrite (mem_range, range_uniq).
-rewrite rcoeffZ rcoeff_polyXn //= Zq.ZModpRing.mulr1.
-rewrite Rq.BasePoly.BigCf.BCA.big_seq_cond Rq.BasePoly.BigCf.BCA.big1 /=; last first.
-+ by rewrite Zq.ZModpRing.addr0.
-move=> j [/mem_range rgj @/predC1 ne_ji].
-rewrite rcoeffZ rcoeff_polyXn // (eq_sym i j) ne_ji /=.
-+ by rewrite Zq.ZModpRing.mulr0.
-qed.
-
-lemma Rpv2RqvE (p : Rp_vec) (i : int) : (Rpv2Rqv p).[i] = Rp2Rq p.[i].
-proof.
-rewrite /Rpv2Rqv /Mat_Rq.Vector."_.[_]" offunvK /vclamp.
-case (0 <= i && i < l) => //; move/(Mat_Rp.Vector.getv_out p i) => ->.
-rewrite /Rp2Rq eq_sym BigRq.XnD1CA.big_seq BigRq.XnD1CA.big1 => //= j /mem_range [ge0_j ltn_j].
-by rewrite rcoeff0 Zp2Zq0 scale0p.
-qed.
-
-lemma Zp2Zq_Zq2Zp_inv (z : Zp) : Zq2Zp (Zp2Zq z) = z.
-proof.
-rewrite /Zq2Zp /Zp2Zq inzmodK modz_small 1: ge0_asint 2:asintK //=.
-rewrite ger0_norm 2:(ltr_le_trans p _ _ (Zp.gtp_asint z)) /p /q; first smt(ge8_q).
-by apply (ler_weexpn2l 2 _ ep eq _); 2: smt(ge2_ep geep1_eq).
-qed.
-
-lemma Rp2Rq_Rq2Rp_inv (p : Rp) : Rq2Rp (Rp2Rq p) = p.
-proof.
-rewrite /Rq2Rp polyXnD1_eqP => i [ge0_i ltn_i].
-rewrite rcoeff_sum /= (BCA.bigD1 _ _  i) /=; 1, 2: by rewrite (mem_range, range_uniq).
-rewrite rcoeffZ rcoeff_polyXn //= Rp2RqE Zp2Zq_Zq2Zp_inv Zp.ZModpRing.mulr1.
-rewrite BCA.big_seq_cond BCA.big1 /=; last by rewrite Zp.ZModpRing.addr0.
-move => j [/mem_range rgj @/predC1 ne_ji].
-by rewrite rcoeffZ rcoeff_polyXn // (eq_sym i j) ne_ji Zp.ZModpRing.mulr0 //.
-qed.
-
-lemma Rpv2Rqv_Rqv2Rpv_inv (pv : Rp_vec) : Rqv2Rpv (Rpv2Rqv pv) = pv.
-proof.
-rewrite /Rqv2Rpv eq_vectorP => i rngi.
-by rewrite {1}/Mat_Rp.Vector."_.[_]" offunvK /vclamp rngi /= Rpv2RqvE Rp2Rq_Rq2Rp_inv.
-qed.
-
-lemma Rq2Rp_DG23 (b : Rp_vec) (s : Rq_vec) : 
-       Rq2Rp (dotp (Rpv2Rqv b) s + h1) = dotp b (Rqv2Rpv s) + Rq2Rp h1.
-proof. by rewrite Rq2Rp_DDl Rq2Rp_DotDl Rpv2Rqv_Rqv2Rpv_inv. qed.
-
-op scaleZq2Zp (z : Zq) : Zp = Zp.inzmod (scale (Zq.asint z) eq ep).
-op scaleZp2Zp (z : Zp) : Zp = Zp.inzmod (scale (Zp.asint z) ep ep).
-op scaleZp2Zppq (z : Zp) : Zppq = Zppq.inzmod (scale (Zp.asint z) ep (2 * ep - eq)).
-op scaleZp2Z2t (z : Zp) : Z2t = Z2t.inzmod (scale (Zp.asint z) ep (et + 1)).
-op scaleZp2Z2 (z : Zp) : Z2 = Z2.inzmod (scale (Zp.asint z) ep 1).
-op scaleZppq2Z2t (z : Zppq) : Z2t = Z2t.inzmod (scale (Zppq.asint z) (2 * ep - eq) (et + 1)).
-
-op scaleRq2Rp (p : Rq) : Rp = 
-  BigRp.XnD1CA.bigi predT (fun (i : int) => scaleZq2Zp p.[i] ** exp Rp.iX i) 0 n.
-op scaleRp2Rp (p : Rp) : Rp = 
-  BigRp.XnD1CA.bigi predT (fun (i : int) => scaleZp2Zp p.[i] ** exp Rp.iX i) 0 n.
-op scaleRp2Rppq (p : Rp) : Rppq = 
-  BigRppq.XnD1CA.bigi predT (fun (i : int) => scaleZp2Zppq p.[i] ** exp Rppq.iX i) 0 n.
-op scaleRp2R2t (p : Rp) : R2t = 
-  BigR2t.XnD1CA.bigi predT (fun (i : int) => scaleZp2Z2t p.[i] ** exp R2t.iX i) 0 n.
-op scaleRp2R2 (p : Rp) : R2 = 
-  BigR2.XnD1CA.bigi predT (fun (i : int) => scaleZp2Z2 p.[i] ** exp R2.iX i) 0 n.
-op scaleRppq2R2t (p : Rppq) : R2t = 
-  BigR2t.XnD1CA.bigi predT (fun (i : int) => scaleZppq2Z2t p.[i] ** exp R2t.iX i) 0 n.
-
-op scaleRqv2Rpv (pv : Rq_vec) : Rp_vec = offunv (fun (i : int) => scaleRq2Rp pv.[i]).
 
 lemma scaleZp2Zp_id (z : Zp) : scaleZp2Zp z = z.
 proof. by rewrite /scaleZp2Zp scale_id 2: Zp.asintK. qed.
@@ -868,6 +634,50 @@ rewrite BCA.big_seq_cond BCA.big1 => /= [j [/mem_range rngj @/predC1 ne_ji] |];
         rewrite scaleZp2Zp_id rcoeffZ rcoeff_polyXn //= ?((eq_sym i j), ne_ji) /=.
 + by apply Zp.ZModpRing.mulr0.
 + by rewrite Zp.ZModpRing.mulr1 Zp.ZModpRing.addr0.
+qed.
+
+lemma scale_comp (x ea eab eb : int):
+      0 <= x => 0 <= eb => eb <= eab => eab <= ea =>
+      scale x ea eb = scale (scale x ea eab) eab eb. 
+proof. 
+(* Context *)
+move=> ge0_x ge0_eb geeb_eab geeab_ea; rewrite /scale /shr. 
+move: (divz_eq x (2^(ea - eb))) 
+      (divz_eq x (2^(ea - eab))) 
+      (divz_eq (x %/ 2 ^ (ea - eab)) (2^(eab - eb))).
+pose dmain := 2 ^ (ea - eb); pose d0 := 2 ^ (ea - eab); pose d1 := 2 ^ (eab - eb).
+pose qmain := x %/ dmain; pose q0 := x %/ d0; pose q1 := x %/ d1.
+pose rmain := x %% dmain; pose r0 := x %% d0; pose r1 := x %% d1.
+move=> divmain div0 div1.
+
+have gt0_d0: 0 < d0.
++ by apply expr_gt0.
+have gt0_d1: 0 < d1.
++ by apply expr_gt0.
+
+have eq_dmain_d0d1: dmain = d0 * d1.
++ rewrite /dmain /d0 /d1 -exprD_nneg. 
+  - by rewrite -(lez_add2r eab 0 (ea - eab)) -addrA /= geeab_ea.
+  - by rewrite -(lez_add2r eb 0 (eab - eb)) -addrA /= geeb_eab.
+  - by congr; rewrite -addzA addKz.
+
+(* Main Proof *)
+move: (euclideU dmain qmain (q0 %/ d1) rmain (q0 %% d1 * d0 + r0)).
++ have <-: x = q0 %/ d1 * dmain + (q0 %% d1 * d0 + r0).
+  - by rewrite eq_dmain_d0d1 (mulzC d0 d1) -(mulzA (q0 %/ d1)) addzA -(mulzDl _ _ d0) -div1.
+rewrite -divmain /=.  
++ have -> /=: 0 <= rmain && rmain < `| dmain |.
+  - split; [by apply /modn_ge0 /ge0_x | move => ge0_rmain].
+    * by rewrite ltz_mod neq_ltz; right; apply expr_gt0.
++ have -> /=:  0 <= q0 %% d1 * d0 + r0 && q0 %% d1 * d0 + r0 < `| dmain |.
+  - split; 1: by apply /addz_ge0 /modn_ge0 /ge0_x /mulr_ge0 /ltzW /gt0_d0 /modz_ge0 /neq_ltz; right.
+    * rewrite ger0_norm eq_dmain_d0d1; first by rewrite mulr_ge0 ltzW.
+      rewrite (ltr_le_trans ((d1 - 1) * d0 + d0) _ (d0 * d1)) 3://.
+      + apply (ler_lt_add _ _ r0 d0); last by apply ltz_pmod.
+        apply /(ler_pmul _ _ d0 d0) /lezz; [by apply /modz_ge0 /neq_ltz; right | by apply ltzW |].
+        by apply (lez_add2l 1); rewrite lez_add1r -addzCA /= ltz_pmod.
+      + by rewrite mulzDl mulNr /= -addzA addNz /= mulzC; apply lezz.
+ by case.
 qed.
 
 lemma scaleZp2Zppq2Z2t_comp (x : Zp) :
@@ -901,28 +711,11 @@ congr; last first.
   by rewrite Zppq.ZModpRing.addr0 Zppq.ZModpRing.mulr1.
 qed.
 
-op Zp2Zppq (z : Zp) : Zppq = Zppq.inzmod (Zp.asint z).
+(* Proof-Specific *)
+lemma Rq2Rp_DG23 (b : Rp_vec) (s : Rq_vec) : 
+       Rq2Rp (dotp (Rpv2Rqv b) s + h1) = dotp b (Rqv2Rpv s) + Rq2Rp h1.
+proof. by rewrite (Rq2Rp_DM (dotp (Rpv2Rqv b) s) h1) Rq2Rp_DotDl Rpv2Rqv_Rqv2Rpv_inv. qed.
 
-op Rp2Rppq (p : Rp) : Rppq =
-  BigRppq.XnD1CA.bigi predT (fun (i : int) => Zp2Zppq p.[i] ** exp Rppq.iX i) 0 n.
-
-lemma Zp2Zppq0 : Zp2Zppq Zp.zero = Zppq.zero.
-proof. by rewrite -eq_inzmod zeroE. qed.
-
-lemma Rp2RppqE (p : Rp) (i : int) : (Rp2Rppq p).[i] = Zp2Zppq p.[i].
-proof.
-case: (i < 0) => [lt0_i|]; first by rewrite !lt0_rcoeff // Zp2Zppq0.
-move/lerNgt=> ge0_i; case: (i < n); last first.
-- by move/lerNgt=> ge_ni; rewrite !gered_rcoeff // Zp2Zppq0.
-move=> lt_in; rewrite rcoeff_sum /= (Rppq.BasePoly.BigCf.BCA.bigD1 _ _ i) /=;
-  1,2: by rewrite (mem_range, range_uniq).
-rewrite rcoeffZ rcoeff_polyXn //= Zppq.ZModpRing.mulr1.
-rewrite Rppq.BasePoly.BigCf.BCA.big_seq_cond Rppq.BasePoly.BigCf.BCA.big1 /=; last first.
-- by rewrite Zppq.ZModpRing.addr0.
-move=> j [/mem_range rgj @/predC1 ne_ji].
-rewrite rcoeffZ rcoeff_polyXn // (eq_sym i j) ne_ji /=.
-- by rewrite Zppq.ZModpRing.mulr0.
-qed.
 
 lemma cmuZq_red23 (z : Zq) (m : Z2) :
       Zp2Zppq ((scaleZq2Zp z) + (Zp.inzmod (shl (Z2.asint m) (2 * ep - eq - 1))))
@@ -931,73 +724,45 @@ lemma cmuZq_red23 (z : Zq) (m : Z2) :
 proof.
 rewrite /Zp2Zppq /Zq2Zp /scaleZq2Zp /scaleZp2Zppq /scale /shr /shl !Zp.inzmodK !modzDm 
         {2}(mulzC 2) -(intmulz ep) mulr2z !opprD !addzA /= (addzC _ eq).
-have ge0_eqep: 0 <= eq - ep; 1: by apply /(lez_trans 1) /(lez_add2l ep); 
-     2: rewrite addzCA /= geep1_eq.
-have leep_eq_ep: eq - ep <= ep; 1: by rewrite -(lez_add2r ep) -addzA /= -mulr2z intmulz mulzC 
-                                               (lez_trans (eq + 1)) 2:geeq1_2ep lez_addl.
-have ge0_2epeq: 0 <= 2 * ep - eq; 1: by rewrite -(lez_add2r eq) -addzA /= (lez_trans (eq + 1)) 
-                                                2:geeq1_2ep lez_addl.
-have leep_2epeq: 2 * ep - eq <= ep; first rewrite mulzC -intmulz mulr2z -(lez_add2l (-ep)) 2!addzA;
-     move: (oppz_le0 (eq - ep)); rewrite ge0_eqep opprD /= addzC => -> //.
-case: (Z2.asint m = 0) => [-> /= | /neq_ltz]; last case => [lt0_m | gt0_m]; 
-      move: (Z2.Sub.valP m) => [ge0_m lt2_m].
-+ by rewrite -Zppq.eq_inzmod -eq_22epeq_ppq /p /q (modz_pow2_div); 
-             [apply Zq.ge0_asint | 
-              split | 
-              rewrite opprD (addzC _ ep) addzA -mulr2z intmulz (mulzC ep) modz_mod modz_dvd_pow].
-+ by rewrite -/Z2.asint lezNgt in ge0_m.
-have -> /= {gt0_m ge0_m lt2_m}: Z2.asint m = 1; first rewrite eqz_leq; split. 
-+ by rewrite -/Z2.asint -lez_add1r -(lez_add2l (-1)) /= in lt2_m.
-+ by rewrite -lez_add1r in gt0_m.
-rewrite -Zppq.eq_inzmod -eq_22epeq_ppq /p modz_dvd_pow; 1: by split.
-rewrite modz_pow2_div; [by apply /addz_ge0 /expr_ge0; 1: apply Zq.ge0_asint | by split |]. 
-rewrite opprD (addzC (-eq)) addzA /= -mulr2z intmulz (mulzC ep) modz_mod divzDr 1: dvdz_exp2l. 
-+ by split => [| ?]; last rewrite -(lez_add2r 1) -(lez_add2l ep) -!addzA /= !addzA addzAC 
-                                   addzC !addzA /= -mulr2z intmulz mulzC geeq1_2ep.
-have -> //: 2 ^ (ep - 1) %/ 2 ^ (eq - ep) = 2 ^ (2 * ep - eq - 1).
-rewrite eq_sym eqz_div 2:dvdz_exp2l 3: -exprD_nneg; last congr; rewrite //#. 
-+ by rewrite neq_ltz; right; apply expr_gt0.
-+ by split => [| ?]; last rewrite -(lez_add2r 1) -(lez_add2l ep) -!addzA /= !addzA 
-                                   addzAC addzC !addzA /= -mulr2z intmulz mulzC geeq1_2ep.
-+ by rewrite -(lez_add2r 1) -addzA /= -(lez_add2r eq) -addzA addzC /= geeq1_2ep.
-+ by apply /(lez_trans 1) /(lez_add2l ep); 2: rewrite addzCA /= geep1_eq.
+case: (Z2.asint m = 0) => [-> /= | /neq_ltz]; last first. 
++ case => [lt0_m | gt0_m]; move: (Z2.Sub.valP m) => [ge0_m lt2_m]; first smt().
+  - have -> /= {gt0_m ge0_m lt2_m}: Z2.asint m = 1 by smt().
+    rewrite -Zppq.eq_inzmod -eq_22epeq_ppq /p modz_dvd_pow; 1: smt(geeq1_2ep geep1_eq).
+    rewrite modz_pow2_div; first 2 smt(Zq.ge0_asint expr_ge0 geeq1_2ep geep1_eq).
+    rewrite opprD (addzC (-eq)) addzA /= -mulr2z intmulz (mulzC ep) modz_mod divzDr 1: dvdz_exp2l.
+    * smt(geeq1_2ep geep1_eq).
+    have -> //: 2 ^ (ep - 1) %/ 2 ^ (eq - ep) = 2 ^ (2 * ep - eq - 1).
+    * by rewrite eq_sym eqz_div 2:dvdz_exp2l 3: -exprD_nneg; 5: congr; smt(geeq1_2ep geep1_eq expr_gt0).
++ rewrite -Zppq.eq_inzmod -eq_22epeq_ppq /p /q modz_pow2_div 1:Zq.ge0_asint.
+  - smt(geeq1_2ep geep1_eq). 
+  - smt(geeq1_2ep geep1_eq modz_dvd_pow). 
 qed.
 
-
-op shl_enc_2 (x : R2, ex : int) : Rp =  
-  BigRp.XnD1CA.bigi predT (fun (i : int) => 
-  Zp.inzmod (shl (Z2.asint x.[i]) ex) ** exp Rp.iX i) 0 n.
-   
-op shl_dec_2 (x : R2t) : Rp =
-  BigRp.XnD1CA.bigi predT (fun (i : int) => 
-  Zp.inzmod (shl (Z2t.asint x.[i]) (ep - et - 1)) ** exp Rp.iX i) 0 n.
-
 lemma cmu_red23 (p : Rq) (m : R2) :
-      Rp2Rppq ((scaleRq2Rp p) + (shl_enc_2 m (2 * ep - eq - 1)))
+      Rp2Rppq ((scaleRq2Rp p) + (shl_enc m (2 * ep - eq - 1)))
       =
-      scaleRp2Rppq ((Rq2Rp p) + (shl_enc_2 m (ep - 1))).
+      scaleRp2Rppq ((Rq2Rp p) + (shl_enc m (ep - 1))).
 proof.
-rewrite polyXnD1_eqP => i rngi.
-rewrite /Rp2Rppq /scaleRp2Rppq.
-rewrite 2!rcoeff_sum /=.
+rewrite polyXnD1_eqP => i rngi; rewrite /Rp2Rppq /scaleRp2Rppq 2!rcoeff_sum /=.
 rewrite !(Rppq.BasePoly.BigCf.BCA.bigD1 _ _ i) /=; first 4 smt(mem_range range_uniq).
 rewrite Rppq.BasePoly.BigCf.BCA.big_seq_cond eq_sym Rppq.BasePoly.BigCf.BCA.big_seq_cond.
 rewrite !Rppq.BasePoly.BigCf.BCA.big1 /= 3:2!Zppq.ZModpRing.addr0 =>
         [j [/mem_range rngj @/predC1 ne_ji] | j [/mem_range rngj @/predC1 ne_ji] |];
         first 2 by rewrite rcoeffZ rcoeff_polyXn // (eq_sym i) ne_ji /= Zppq.ZModpRing.mulr0.
-rewrite 2!rcoeffZ rcoeff_polyXn //= 2!Zppq.ZModpRing.mulr1.
-rewrite /Rq2Rp /shl_enc_2. rewrite -BigRp.XnD1CA.big_split /=.
-rewrite rcoeff_sum /=.
+rewrite 2!rcoeffZ rcoeff_polyXn //= 2!Zppq.ZModpRing.mulr1 /Rq2Rp /shl_enc_2. 
+rewrite -BigRp.XnD1CA.big_split rcoeff_sum (BCA.bigD1 _ _ i) /=; first 2 smt(mem_range range_uniq).
+rewrite BCA.big_seq_cond BCA.big1 2:Zp.ZModpRing.addr0 => 
+        [j [/mem_range rngj @/predC1 ne_ji]|] /=.
++ by rewrite rcoeffD 2!rcoeffZ rcoeff_polyXn // (eq_sym i) ne_ji /= 
+             2!Zp.ZModpRing.mulr0 Zp.ZModpRing.addr0.
+rewrite rcoeffD 2!rcoeffZ !rcoeff_polyXn //= 2!Zp.ZModpRing.mulr1 
+        /scaleRq2Rp -BigRp.XnD1CA.big_split rcoeff_sum.
 rewrite (BCA.bigD1 _ _ i) /=; first 2 smt(mem_range range_uniq).
-rewrite BCA.big_seq_cond BCA.big1 2:Zp.ZModpRing.addr0 => [j [/mem_range rngj @/predC1 ne_ji]|] /=.
-by rewrite rcoeffD 2!rcoeffZ !rcoeff_polyXn // (eq_sym i) ne_ji /= 2!Zp.ZModpRing.mulr0 Zp.ZModpRing.addr0.
-rewrite rcoeffD 2!rcoeffZ !rcoeff_polyXn //= 2!Zp.ZModpRing.mulr1.
-rewrite /scaleRq2Rp -BigRp.XnD1CA.big_split /= rcoeff_sum /=.
-rewrite (BCA.bigD1 _ _ i) /=; first 2 smt(mem_range range_uniq).
-rewrite BCA.big_seq_cond BCA.big1 2:Zp.ZModpRing.addr0 => [j [/mem_range rngj @/predC1 ne_ji]|] /=.
-by rewrite rcoeffD 2!rcoeffZ !rcoeff_polyXn // (eq_sym i) ne_ji /= 2!Zp.ZModpRing.mulr0 Zp.ZModpRing.addr0.
-rewrite rcoeffD 2!rcoeffZ !rcoeff_polyXn //= 2!Zp.ZModpRing.mulr1.
-by rewrite eq_sym; apply cmuZq_red23.
+rewrite BCA.big_seq_cond BCA.big1 2:Zp.ZModpRing.addr0 => 
+        [j [/mem_range rngj @/predC1 ne_ji]|] /=.
++ by rewrite rcoeffD 2!rcoeffZ !rcoeff_polyXn // (eq_sym i) ne_ji /= 
+             2!Zp.ZModpRing.mulr0 Zp.ZModpRing.addr0.
+by rewrite rcoeffD 2!rcoeffZ !rcoeff_polyXn //= 2!Zp.ZModpRing.mulr1 cmuZq_red23.
 qed.
 
 (* ------------------------------------------------------------------------------------- *)
@@ -1022,7 +787,7 @@ module Saber_PKE_Scheme : Scheme = {
       sd <$ dseed;
       _A <- gen sd;
       s <$ dsmallRq_vec;
-      b <- scale_vec_Rq_Rp (_A *^ s + h);
+      b <- scaleRqv2Rpv (_A *^ s + h);
       
       return (pk_encode (sd, b), sk_encode s);
    }
@@ -1044,9 +809,9 @@ module Saber_PKE_Scheme : Scheme = {
       b <- pk_dec.`2;
       _A <- gen sd;
       s' <$ dsmallRq_vec;
-      b' <- scale_vec_Rq_Rp ((trmx _A) *^ s' + h);
-      v' <- (dotp b (mod_p_Rq_vec s')) + (mod_p_Rq h1);
-      cm <- scale_Rp_R2t (v' + (shl_enc m_dec (ep - 1)));
+      b' <- scaleRqv2Rpv ((trmx _A) *^ s' + h);
+      v' <- (dotp b (Rqv2Rpv s')) + (Rq2Rp h1);
+      cm <- scaleRp2R2t (v' + (shl_enc m_dec (ep - 1)));
       
       return c_encode (cm, b');
    }
@@ -1063,8 +828,8 @@ module Saber_PKE_Scheme : Scheme = {
       s <- sk_decode sk;
       cm <- c_dec.`1;
       b' <- c_dec.`2;
-      v <- (dotp b' (mod_p_Rq_vec s)) + (mod_p_Rq h1);
-      m' <- scale_Rp_R2 (v  - (shl_dec cm) + (mod_p_Rq h2));
+      v <- (dotp b' (Rqv2Rpv s)) + (Rq2Rp h1);
+      m' <- scaleRp2R2 (v  - (shl_dec cm) + (Rq2Rp h2));
       
       return Some (m_encode m');
    }
